src/crypto/loopunroll/bitshiftlemmas.dfy
@@ -1,0 +1,43 @@
+include "../../lib/util/types.s.dfy"
+include "../../lib/util/operations.s.dfy"
+include "../../lib/util/words_and_bytes.s.dfy"
+include "../../lib/collections/Seqs.s.dfy"
+include "../../arch/x64/def.s.dfy"
+include "../../arch/x64/vale.i.dfy"
+include "../../lib/util/dafny_wrappers.i.dfy"
+
+// This really shows that bitvectors are not going to work well for
+// us as fundamental representation in Dafny. Dafny is missing a
+// translation of bv[i..j] into Z3 extract for a start.
+// Other simple lemmas of conversion don't prove for example
+// at sizes of 16.
+
+module bitvectorsasfoundation {
+
+import opened x64_def_s
+import opened types_s
+import opened x64_vale_i
+import opened dafny_wrappers_i
+
+lemma lemma_bv128_conversion(x : bv128)
+  ensures (x as uint128) as bv128 == x;
+{ if (x == 0) {
+ }
+  else {
+    lemma_bv128_conversion(x >> 1);
+  }
+}
+
+/*
+lemma lemma_bv128_shr_zero(x : bv128)
+  ensures x >> 0 == x;
+{}
+
+lemma {:timeLimitMultiplier 3} lemma_uint128_shr_zero(x : uint128)
+  ensures ((x as bv128) >> 0) as uint128 == x;
+{
+  lemma_bv128_shr_zero(x as bv128);
+}
+*/
+
+}
