src/crypto/loopunroll/bvvsuintvsquadword.dfy
@@ -1,0 +1,204 @@
+include "../../lib/util/types.s.dfy"
+include "../../lib/util/operations.s.dfy"
+include "../../lib/util/words_and_bytes.s.dfy"
+include "../../lib/collections/Seqs.s.dfy"
+include "../../arch/x64/def.s.dfy"
+include "../../arch/x64/vale.i.dfy"
+
+// What are reasonable experiments to tell if we can specify things
+// in which datatype to prove properties of carryless multiply?
+
+module bvvsuintvsquadword {
+
+import opened x64_def_s
+import opened types_s
+import opened x64_vale_i
+
+/*
+lemma lemma_bv64_is_zero_or_64_shifts_gives_zero(b : bv64)
+  ensures b == 0 || (b << 64) == 0;
+{
+}
+
+lemma lemma_bv64_is_zero_or_upto_64_shifts_gives_zero(b : bv64)
+  ensures b == 0 || exists i : nat :: i <= 64 ==> b << i == 0; 
+{
+  if (b == 0) {
+  } else {
+    lemma_bv64_is_zero_or_64_shifts_gives_zero(b);
+    assert 64 <= 64;
+  }
+}
+*/
+
+// BV version proves.
+function BV_CL_MUL_SHIFT'(i : nat, a : bv64, b : bv64, r : bv128) : bv128
+  requires 0 <= i <= 64;
+  decreases 64 - i;
+{
+ if (b << i) != 0 then
+   if ((a & 1) != 0) then
+     BV_CL_MUL_SHIFT'(i + 1, a >> 1, b, r ^ ((b << i) as bv128))
+   else 
+     BV_CL_MUL_SHIFT'(i + 1, a >> 1, b, r)
+ else 
+  r
+}
+
+function BV_CL_MUL_SHIFT(a : bv64, b : bv64) : bv128
+{
+ BV_CL_MUL_SHIFT'(0, a, b, 0 as bv128)
+}
+
+
+function bit64(v : bv64, i : nat) : bv1
+  requires i < 64;
+{
+  ((v >> i) & 0x1) as bv1
+}
+
+/* 
+//Prove
+lemma lemma_bit64_check63()
+  ensures bit64(0x8000_0000_0000_0000,63) == 0x1;
+{}
+
+lemma lemma_bit64_check0()
+  ensures bit64(0x1,0) == 0x1;
+{}
+
+lemma lemma_bit64_check_zeros()
+  ensures forall i : nat :: i < 64 ==> bit64(0x0,i) == 0x0;
+{}
+
+lemma lemma_bit64_check_ones_fixed(i : nat)
+  requires i < 64;
+  ensures  bit64(0xFFFF_FFFF_FFFF_FFFF,i) == 0x1;
+{}
+*/
+
+/* Won't prove reasonably.
+lemma {:timeLimitMultiplier 3} lemma_bit64_check_ones()
+  ensures forall i : nat :: i < 64 ==> bit64(0xFFFF_FFFF_FFFF_FFFF,i) == 0x1;
+{
+  forall j : nat | j < 64
+   ensures forall i : nat :: i < 64 ==> bit64(0xFFFF_FFFF_FFFF_FFFF,i) == 0x1;
+ {
+   lemma_bit64_check_ones_fixed(j);
+ }
+}
+*/
+
+function bit128(v : bv128, i : nat) : bv1
+  requires i < 128;
+{
+  ((v >> i) & 0x1) as bv1
+}
+
+lemma lemma_bit128_check127()
+  ensures bit128(0x8000_0000_0000_0000_0000_0000_0000_0000, 127) == 0x1;
+{}
+
+lemma lemma_bit128_check0()
+  ensures bit128(0x1,0) == 0x1;
+{}
+
+lemma lemma_bit128_check_zeros()
+  ensures forall i : nat :: i < 128 ==> bit128(0x0,i) == 0x0;
+{}
+
+/*
+lemma {:timeLimitMultiplier 3} lemma_bit128_check_ones_fixed(i : nat)
+  requires i < 128;
+  ensures  bit128(0xFFFF_FFFF_FFFF_FFFF_FFFF_FFFF_FFFF_FFFF,i) == 0x1;
+{}
+
+lemma {:timeLimitMultiplier 3} lemma_bit128_check_ones()
+  ensures forall i : nat :: i < 128 ==> bit128(0xFFFF_FFFF_FFFF_FFFF_FFFF_FFFF_FFFF_FFFF,i) == 0x1;
+{
+  forall j : nat | j < 128
+   ensures forall i : nat :: i < 128 ==> bit128(0xFFFF_FFFF_FFFF_FFFF_FFFF_FFFF_FFFF_FFFF,i) == 0x1;
+ {
+   lemma_bit128_check_ones_fixed(j);
+ }
+}
+*/
+
+// From Gueron and Kounavis, 2014.
+function bvclmullow(j : nat, i : nat, a : bv64, b : bv64) : bv1
+  requires j <= i;
+  requires i < 64;
+  decreases i - j;
+{
+  if (j == i) then
+    bit64(a,j) ^ bit64(b, i - j)
+  else 
+    bit64(a,j) ^ bit64(b, i - j) ^ bvclmullow(j + 1, i, a, b)
+}
+
+function bvclmulhigh(i :nat, j : nat, a : bv64, b : bv64) : bv1
+  requires i - (64 - 1) <= j <= 64 - 1;
+  requires 64 <= i <= 126;
+  decreases 64 - 1 - j;
+{
+  if (j == 64 - 1) then
+    bit64(a,j) ^ bit64(b, i - j)
+  else 
+    bit64(a, j) ^ bit64(b, i - j) ^ bvclmulhigh(i, j + 1, a, b)
+}
+
+predicate bvclmul(a : bv64, b : bv64, c : bv128)
+{  
+  forall i : nat :: i < 63       ==> bit128(c,i) == bvclmullow(0, i, a, b) &&
+  forall i : nat :: 64 <= i <= 126 ==> bit128(c,i) == bvclmulhigh(i, i - 64 + 1, a, b) &&
+  bit128(c,127) == 0
+}
+
+// No way this proves of course.
+//lemma {:timeLimitMultiplier 10} BV_CL_MUL_SHIFT_IS_bvclmul_zero()
+//  ensures bvclmul(0,0, BV_CL_MUL_SHIFT(0,0));
+//{}
+
+
+/* Not proving.
+// uint version
+function power(b:int, e:nat) : int
+    decreases e;
+{
+    if (e==0) then
+        1
+    else
+        b*power(b,e-1)
+}
+
+function uint64Shl(v : uint64, i : nat) : uint64
+{
+  (v * power(2,i)) % 0x1_0000_0000_0000_0000
+}
+
+function uint64Shr1(v : uint64) : uint64
+{
+  (v / 2)
+}
+
+function {:timeLimitMultiplier 6} UINT64_CL_MUL_SHIFT'(i : nat, a : uint64, b : uint64, r : bv128) : bv128
+  requires 0 <= i <= 64;
+  decreases 64 - i;
+{
+ if (uint64Shl(b, i)) != 0 then
+   if ((a % 2) != 0) then
+     UINT64_CL_MUL_SHIFT'(i + 1, uint64Shr1(a), b, r ^ ((uint64Shl(b,i)) as bv128))
+   else 
+     UINT64_CL_MUL_SHIFT'(i + 1, uint64Shr1(a), b, r)
+ else 
+  r
+}
+
+function UINT64_CL_MUL_SHIFT(a : uint64, b : uint64) : bv128
+{
+  UINT64_CL_MUL_SHIFT'(0, a, b, 0 as bv128)
+}
+*/
+
+
+}
